
\documentclass{article}
\usepackage{amsmath, amssymb, graphics, setspace}

\newcommand{\mathsym}[1]{{}}
\newcommand{\unicode}[1]{{}}

\newcounter{mathematicapage}
\begin{document}


\[\frac{\partial \left(\frac{A_1 \left(1-\frac{1}{e^ {-(\nu-\omega )}+1}\right)+\frac{A_2}{e^ {-(\nu-\omega )}+1}}{d}-\nu+y_1\right)}{\partial
\nu}=\frac{\frac{A_2 e^{\omega -\nu}}{\left(e^{\omega -\nu}+1\right)^2}-\frac{A_1 e^{\omega -\nu}}{\left(e^{\omega -\nu}+1\right)^2}}{d}-1\]

The first order conditions lead to
%used the following in wolfram alpha for first order conditions
% solve  (-(A1 e^(-x + ω))/(1 + e^(-x + ω))^2 + (A2 e^(-x + ω))/(1 + e^(-x + ω))^2)/d=1 for x
$e^x = \frac{(A_2-A_1) e^{\omega}}{2d}-e^{\omega}-e^\omega \sqrt{(\frac{A_2-A_1}{2d}-1)^2-1}$
or
$e^{x-\omega} = \frac{(A_2-A_1) }{2d}-1- \sqrt{(\frac{A_2-A_1}{2d}-1)^2-1}$

For the richer consumer, 

%For richer consumer
%  d(y2-x +(1/delta)*((1-(1/(1+exp(-(x-lambda)))))* A1 + (1/(1+exp(-(x-lambda))))*A2))/dx

\[\frac{\partial (\frac{A_1 (1-\frac{1}{e^ {-(\nu-\lambda )}+1})+\frac{A_2}{e^ {-(\nu-\lambda )}+1}}{d}-\nu+y_2)}{\partial
\nu}=\frac{(A_2-A_1) e^{\lambda -\nu}}{d\times(e^{\lambda -\nu}+1)^2}-1\]

The first conditions for the richer consumer are similarly based on $\underline{\lambda}$.

% the solution can be arrived at using wolfram with
% solve  (-(A1 e^(-x + λ))/(1 + e^(-x + λ))^2 + (A2 e^(-x + λ))/(1 + e^(-x + λ))^2)/δ=1 for x

\end{document}